# Ch.1

**Complex numbers:**  $C: \{a + bi, a,b\in R\}$ 

**Addition & multiplication on $C$**

 **Properties of arithmetic on $C$**:



**Example 2.4**: 

Prove $ab = ba, \forall a,b \in C$



**Notation $F: R \cup C$**



$R^2, R^3: \{(x,y)\}, \{(x,y,z)\}$



**List and Sets**:

 **List**: $(3,5) \neq (5,3), (4) \neq (4,4) \neq (4,4,4)$ 

**Sets**: $\{3,5\} = \{5,3\}, \{4\} = \{4,4\} = \{4,4,4\}$



**Notation** $F^n : \{(x_1,...,x_n), x_j \in F, j = 1,...,n\}$

 

**Addition in $F_n$**: $(x_1, ...,x_n) + (y_1,...,y_n) = (x_1+y_1,...,x_n + y_n)$

$x,y\in F^n, x+y = y+x$



**Definition of 0**: $0 = (0, ..., 0)$ (length $n$)

**Additive inverse in $F^n$**: $x + (-x) = 0$

**Scalar multiplication in $F^n$**: $\lambda (x_1, ...,x_n) = (\lambda x_1,...,\lambda x_n)$



**Field**: A set containing at least two distinct elements $\{0, 1\}$ 

## 1.B

**Vector space** comes from properties of **addition** and **scalar** **multiplication** in $F^n$

 e.g. $V$ is a **vector space** over $F$;  $R^n$ is a vector space over $R$.

**Set of functions**: $F^S: S \to F$

**Sum of $f, g, \forall f,g\in F^S$ **: $f+g \in F^S: (f+g)(x) = f(x) + g(x)$

**Product**: $\lambda \in F, f \in F^S, \lambda f \in F^S$: $(\lambda f)(x) = \lambda f(x) | \forall x \in S$

**Definition of vector space of $F^S$**: 

1. *Additive identity*: $f_0: S \to F, f_0(x) = 0$
2. *Additive inverse*: $-f(x) = -f(x), \forall x \in S$

**Unique Additive identity** : Suppose $0, 0'$ are both addictive identities for $V$

$0 = 0 + 0' = 0'+0 = 0' \implies 0 = 0'$

**Unique additive inverse**: Suppose $V$ is a vector space and $v \in V$, suppose $w , w'$ are additive inverse of $v$

$\implies w = w + 0 = w + (w + v) = w + (w' + v) = w' + (w + v) = w' + 0 = w'$

**Define $-v, w-v$**: $-v$ is the additive inverse of $v$, $w - v = w + (-v)$ 

**The number 0 times a vector**: 

$0v = (0+0)v = 0v + 0v \implies 0v + (- 0v) = 0v + 0v + (- 0v) \implies 0v = 0$\

\



\

\



   76776ytyytytyr\\\\\

\\\\\\\\\\\\\\\\\\\\\\\\\\\\\\\\

 ``   ` ` ` ` ` ` ` ` `  ` ` ` ` ` `                    n  bjhjbhjhbhjbh               `

**The number $a$ times the v       `tor 0**: 

$a0 = a(0+0) = a0 + a0 \implies a0-a0 = a0 + a0-a0 \implies 0 = a0$

**The number -1 times a vector $v$**:``````````````````````````````````````````````````````````````````````````````````````````````````` 





$-1 v + 2v = (-1+2)v = v \implies -1v + 2v - 2v = v-2v \implies -1v = v - 2v $

$\implies -1v + 1v = v - 2v + 1v = 0 \implies v + (-2+1)v = 0 \implies v + -1v = 0$

*Suppose the Additive inverse of $v$ is $-v$* $\implies v + (-v) = 0 = v + -1v \implies -v = -1v$









